pure_model/ZBA-rewrites.lean
@@ -1,0 +1,65 @@
+import LeanRV64DLEAN.Sail.Sail
+import LeanRV64DLEAN.Sail.BitVec
+import LeanRV64DLEAN.Defs
+import LeanRV64DLEAN.Specialization
+import LeanRV64DLEAN.RiscvExtras
+-- added the imports bellow, had to move pure_func to the library folder
+import LeanRV64DLEAN
+import LeanRV64DLEAN.pure_func
+
+open Functions
+open Retired
+open Sail
+open PureFunctions
+
+-- ZBA extensions
+
+-- shifts unsigned word by some specifc amount and adds rs2_val
+theorem execute_ZBA_RTYPEUW_pure64_RISCV_ADDUW (rs2_val : BitVec 64) (rs1_val : BitVec 64) :
+    execute_ZBA_RTYPEUW_pure64 rs2_val rs1_val bropw_zba.RISCV_ADDUW
+      = BitVec.zeroExtend 64 (BitVec.extractLsb 31 0 rs1_val) <<< 0#2 + rs2_val
+       := by
+  unfold execute_ZBA_RTYPEUW_pure64
+  simp
+  unfold shift_bits_left Sail.BitVec.extractLsb zero_extend Sail.BitVec.zeroExtend HPow.hPow instHPowInt_leanRV64DLEAN
+  simp only [Int.reduceToNat, Int.reducePow, Int.reduceMul, BitVec.truncate_eq_setWidth,
+    BitVec.shiftLeft_eq', BitVec.toNat_ofNat, Nat.reducePow, Nat.zero_mod, BitVec.shiftLeft_zero]
+
+theorem execute_ZBA_RTYPEUW_pure64_RISCV_SH1ADDUW (rs2_val : BitVec 64) (rs1_val : BitVec 64) :
+    execute_ZBA_RTYPEUW_pure64 rs2_val rs1_val bropw_zba.RISCV_SH1ADDUW
+      = BitVec.zeroExtend (Int.toNat 64) (BitVec.extractLsb 31 0 rs1_val) <<< 1#2 + rs2_val
+  := by
+  unfold execute_ZBA_RTYPEUW_pure64
+  simp
+  unfold shift_bits_left Sail.BitVec.extractLsb zero_extend Sail.BitVec.zeroExtend HPow.hPow instHPowInt_leanRV64DLEAN
+  rfl
+
+theorem execute_ZBA_RTYPEUW_pure64_RISCV_SH2ADDUW (rs2_val : BitVec 64) (rs1_val : BitVec 64) :
+    execute_ZBA_RTYPEUW_pure64 rs2_val rs1_val bropw_zba.RISCV_SH2ADDUW
+      = BitVec.zeroExtend (Int.toNat 64) (BitVec.extractLsb 31 0 rs1_val) <<< 2#2 + rs2_val
+  := by
+  unfold execute_ZBA_RTYPEUW_pure64
+  simp
+  unfold shift_bits_left Sail.BitVec.extractLsb zero_extend Sail.BitVec.zeroExtend HPow.hPow instHPowInt_leanRV64DLEAN
+  rfl
+
+theorem execute_ZBA_RTYPEUW_pure64_RISCV_SH3ADDUW (rs2_val : BitVec 64) (rs1_val : BitVec 64) :
+    execute_ZBA_RTYPEUW_pure64 rs2_val rs1_val bropw_zba.RISCV_SH3ADDUW
+      = BitVec.zeroExtend (Int.toNat 64) (BitVec.extractLsb 31 0 rs1_val) <<< 3#2 + rs2_val
+  := by
+  unfold execute_ZBA_RTYPEUW_pure64
+  simp
+  unfold shift_bits_left Sail.BitVec.extractLsb zero_extend Sail.BitVec.zeroExtend HPow.hPow instHPowInt_leanRV64DLEAN
+  rfl
+
+theorem execute_ZBA_RTYPE_pure64_RISCV_SH1ADD (rs2_val : BitVec 64) (rs1_val : BitVec 64) :
+    execute_ZBA_RTYPE_pure64 rs2_val rs1_val brop_zba.RISCV_SH1ADD
+    = BitVec.add (rs1_val <<< 1#2) rs2_val := by rfl
+
+theorem execute_ZBA_RTYPE_pure64_RISCV_SH2ADD (rs2_val : BitVec 64) (rs1_val : BitVec 64) :
+    execute_ZBA_RTYPE_pure64 rs2_val rs1_val brop_zba.RISCV_SH2ADD
+    = BitVec.add (rs1_val <<< 2#2) rs2_val:= by rfl
+
+theorem execute_ZBA_RTYPE_pure64_RISCV_SH3ADD(rs2_val : BitVec 64) (rs1_val : BitVec 64) :
+    execute_ZBA_RTYPE_pure64 rs2_val rs1_val brop_zba.RISCV_SH3ADD
+    = BitVec.add (rs1_val <<< 3#2) rs2_val:= by rfl
