pure_model/ZBB-rewrites.lean
@@ -1,0 +1,58 @@
+import LeanRV64DLEAN.Sail.Sail
+import LeanRV64DLEAN.Sail.BitVec
+import LeanRV64DLEAN.Defs
+import LeanRV64DLEAN.Specialization
+import LeanRV64DLEAN.RiscvExtras
+-- added the imports bellow, had to move pure_func to the library folder
+import LeanRV64DLEAN
+import LeanRV64DLEAN.pure_func
+
+open Functions
+open Retired
+open Sail
+open PureFunctions
+
+-- SIMPLIFICATION OF RISC-V EXTENSION, had to translate into bit vec form
+
+-- ZBB EXTENSION
+theorem execute_ZBB_RTYPEW_pure64_RISCV_ROLW (rs2_val : BitVec 64) (rs1_val : BitVec 64) :
+  execute_ZBB_RTYPEW_pure64 rs2_val rs1_val bropw_zbb.RISCV_ROLW
+    = BitVec.signExtend 64
+    (BitVec.setWidth 32 rs1_val <<< BitVec.extractLsb 4 0 rs2_val |||
+      BitVec.setWidth 32 rs1_val >>>
+        (BitVec.extractLsb' 0 (BitVec.length (BitVec.extractLsb 4 0 rs2_val))
+            (BitVec.ofInt (0 + BitVec.length (BitVec.extractLsb 4 0 rs2_val) + 1)
+              ((BitVec.length (BitVec.setWidth 32 rs1_val)))) -
+          BitVec.extractLsb 4 0 rs2_val))
+     := by rfl
+
+--TO DO ASK IF INSTANCE IS CORRECT BV UNSURE
+theorem execute_ZBB_RTYPEW_pure64_RISCV_RORW(rs2_val : BitVec 64) (rs1_val : BitVec 64) :
+  execute_ZBB_RTYPEW_pure64 rs2_val rs1_val bropw_zbb.RISCV_RORW
+    = BitVec.signExtend (2 ^ 3 * 8)
+    (BitVec.setWidth 32 rs1_val >>> (rs2_val.toNat % 32) |||
+      BitVec.setWidth 32 rs1_val <<<
+        ((2 ^ BitVec.length (BitVec.extractLsb 4 0 rs2_val) - rs2_val.toNat % 32 +
+            BitVec.length (BitVec.setWidth 32 rs1_val) % 2 ^ (BitVec.length (BitVec.extractLsb 4 0 rs2_val) + 1)) %
+          2 ^ BitVec.length (BitVec.extractLsb 4 0 rs2_val)))
+     := by
+    unfold execute_ZBB_RTYPEW_pure64
+    simp
+    unfold sign_extend Sail.BitVec.signExtend rotate_bits_right shift_bits_right Sail.BitVec.extractLsb shift_bits_left to_bits get_slice_int
+    simp
+    --unfold HOr.hOr instHOrBitVec_leanRV64DLEAN
+    --simp
+    rfl
+
+-- extract byte or halfwords and either sign or zero extend it
+theorem execute_ZBB_EXTOP_pure64_RISCV_SEXTB (rs1_val : BitVec 64) :
+    execute_ZBB_EXTOP_pure64 rs1_val extop_zbb.RISCV_SEXTB
+      = BitVec.signExtend 64 (BitVec.extractLsb 7 0 rs1_val) := by rfl
+
+theorem execute_ZBB_EXTOP_pure64_RISCV_SEXTH (rs1_val : BitVec 64) :
+    execute_ZBB_EXTOP_pure64 rs1_val extop_zbb.RISCV_SEXTH
+      = BitVec.signExtend 64 (BitVec.extractLsb 15 0 rs1_val)  := by rfl
+
+theorem execute_ZBB_EXTOP_pure64_RISCV_ZEXTH (rs1_val : BitVec 64) :
+    execute_ZBB_EXTOP_pure64 rs1_val extop_zbb.RISCV_ZEXTH
+      = BitVec.zeroExtend 64 (BitVec.extractLsb 15 0 rs1_val) := by rfl
