pure_model/examples.lean
@@ -1,0 +1,48 @@
+
+ /-simp
+  simp [Functions.xlen]
+  have h1 : (2 : Int) * (2 ^(3 : Int) * 8) = 128 := by rfl --such that types match
+  rw [h1]
+  simp
+  unfold to_bits
+  unfold get_slice_int
+  simp [Sail.BitVec.extractLsb]
+  simp [BitVec.extractLsb]
+  simp [extractLsb'_extractLsb'2]
+  --rw [BitVec.setWidth_eq]
+  --dsimp [BitVec.setWidth_eq]
+  simp [extractLsb'_zero]
+  rw [BitVec.setWidth_setWidth]
+  · rfl -- how to do case distinctions
+  · omega -- used to proof omega terms
+ example rewrites
+
+     --have x : ((2:Int) ^ (3:Int) * 8).toNat = 64 := rfl
+      --dsimp!
+      --intros
+
+-- in this file we are trying to proof some simple potential peephole rewrites
+/-
+example (f : BitVec 32 -> BitVec 32) (x : α) (h : α = BitVec 32) (y : BitVec 32) :
+    f y = y := by
+  rw [← h] at y
+
+--@[simp]
+theorem foo :  execute_MUL_pure64 { high := false, signed_rs1 := false, signed_rs2 := false } 0#64 1#64 = 0#64 := by
+  sorry
+  --unfold execute_MUL_pure64
+  --simp
+  --simp [Functions.xlen]
+  --have h1 : (2 : Int) * (2 ^(3 : Int) * 8) = 128 := by rfl
+  --rw [h1]
+  --have h2 :  ((2 : Int) ^(3 : Int) * 8 -1) = 63 := by rfl
+  --simp only [Int.reduceToNat, to_bits, get_slice_int, Nat.reduceAdd, Int.toNat_zero,
+    --Int.Nat.cast_ofNat_Int, BitVec.ofInt_ofNat, BitVec.reduceExtracLsb']
+  --simp only [Sail.BitVec.extractLsb, BitVec.extractLsb_ofNat, Nat.reducePow,
+    --Nat.zero_mod, Nat.shiftRight_zero]
+  --rfl
+-- #print axioms foo
+-/
+
+
+    -/
