pure_model/proofsBVDecide.lean
@@ -1,0 +1,26 @@
+import LeanRV64DLEAN.Sail.Sail
+import LeanRV64DLEAN.Sail.BitVec
+import LeanRV64DLEAN.Defs
+import LeanRV64DLEAN.Specialization
+import LeanRV64DLEAN.RiscvExtras
+import LeanRV64DLEAN
+import LeanRV64DLEAN.pure_func
+open Functions
+open Retired
+open Sail
+open PureFunctions
+
+-- COLLECTION OF PROOFS THAT CAN BE DONE WITH BV_DECIDE VERY SMOOTHLY AND NOT WITH RFL ETC.
+
+--1. using Bv_decide
+theorem execute_RTYPE_pure64__RISCV_AND (rs2_val : BitVec 64) (rs1_val : BitVec 64)  : PureFunctions.execute_RTYPE_pure64 rop.RISCV_AND rs2_val rs1_val
+    = BitVec.and rs2_val rs1_val := by
+  unfold PureFunctions.execute_RTYPE_pure64
+  bv_decide
+
+-- 1. no possible by rfl etc
+theorem execute_RTYPE_pure64__RISCV_AND1 (rs2_val : BitVec 64) (rs1_val : BitVec 64)  : PureFunctions.execute_RTYPE_pure64 rop.RISCV_AND rs2_val rs1_val
+    = BitVec.and rs2_val rs1_val := by
+  unfold PureFunctions.execute_RTYPE_pure64
+  --rfl
+  sorry 
