pure_model/uglyproofs.lean
@@ -1,0 +1,90 @@
+import LeanRV64DLEAN.Sail.Sail
+import LeanRV64DLEAN.Sail.BitVec
+import LeanRV64DLEAN.Defs
+import LeanRV64DLEAN.Specialization
+import LeanRV64DLEAN.RiscvExtras
+import LeanRV64DLEAN
+import LeanRV64DLEAN.pure_func
+open Functions
+open Retired
+open Sail
+open PureFunctions
+
+
+-- 1. ugly
+theorem execute_RTYPE_pure64__RISCV_SLTU (rs2_val : BitVec 64) (rs1_val : BitVec 64) :
+    PureFunctions.execute_RTYPE_pure64 (rop.RISCV_SLTU) (rs2_val : (BitVec 64)) (rs1_val : (BitVec 64)) =
+      let immext : BitVec 64 := (BitVec.signExtend (((2 ^ 3) * 8)) imm);
+      let b := BitVec.ult rs1_val rs2_val;
+      BitVec.setWidth 64 (BitVec.ofBool b)  := by
+  unfold PureFunctions.execute_RTYPE_pure64
+  simp
+  unfold zero_extend Sail.BitVec.zeroExtend bool_to_bits bool_bits_forwards zopz0zI_u
+  rfl
+
+-- 1. nice rewrite
+  theorem execute_RTYPE_pure64__RISCV_SLTU1 (rs2_val : BitVec 64) (rs1_val : BitVec 64) :
+    PureFunctions.execute_RTYPE_pure64 (rop.RISCV_SLTU) (rs2_val : (BitVec 64)) (rs1_val : (BitVec 64)) =
+      let immext : BitVec 64 := (BitVec.signExtend (((2 ^ 3) * 8)) imm);
+      let b := BitVec.ult rs1_val rs2_val;
+      BitVec.setWidth 64 (BitVec.ofBool b)  := by rfl
+
+--2. longer proof before having the instance simp lemma that rewrote the instances
+theorem execute_ITYPE_pure64_RISCV_ADDI (imm : BitVec 12) (rs1_val : BitVec 64) : PureFunctions.execute_ITYPE_pure64 imm rs1_val iop.RISCV_ADDI
+    = let immext : BitVec 64 := (BitVec.signExtend (((2 ^ 3) * 8)) imm) ;
+    BitVec.add rs1_val immext := by
+unfold PureFunctions.execute_ITYPE_pure64
+simp
+unfold sign_extend Sail.BitVec.signExtend HPow.hPow instHPowInt_leanRV64DLEAN
+bv_decide
+
+
+--2 after having the simp lemma
+
+@[simp] theorem sail_hPow_eq (x y : Int) : x ^ y  = x ^ y.toNat := by rfl
+
+theorem execute_ITYPE_pure64_RISCV_ADDI1 (imm : BitVec 12) (rs1_val : BitVec 64) : PureFunctions.execute_ITYPE_pure64 imm rs1_val iop.RISCV_ADDI
+    = let immext : BitVec 64 := (BitVec.signExtend (((2 ^ 3) * 8)) imm) ;
+    BitVec.add rs1_val immext := by
+unfold PureFunctions.execute_ITYPE_pure64
+simp
+unfold sign_extend Sail.BitVec.signExtend --HPow.hPow instHPowInt_leanRV64DLEAN
+bv_decide
+
+--3 proof where we need to unfold to use bv_decide while rfl directly sees it
+theorem execute_ITYPE_pure64_RISCV_ANDI_bv (imm : BitVec 12) (rs1_val : BitVec 64) :
+    PureFunctions.execute_ITYPE_pure64 imm rs1_val  iop.RISCV_ANDI
+      = let immext : BitVec 64 := (BitVec.signExtend (((2 ^ 3) * 8)) imm);
+      BitVec.and rs1_val immext := by
+        unfold PureFunctions.execute_ITYPE_pure64
+        simp
+        unfold sign_extend Sail.BitVec.signExtend  HAnd.hAnd instHAndBitVec_leanRV64DLEAN instHAndOfAndOp
+        bv_decide
+    -- vs rfl directly can be applied -> generalizes to all logical bit vec operations
+  theorem execute_ITYPE_pure64_RISCV_ANDI_rfl (imm : BitVec 12) (rs1_val : BitVec 64) :
+    PureFunctions.execute_ITYPE_pure64 imm rs1_val  iop.RISCV_ANDI
+      = let immext : BitVec 64 := (BitVec.signExtend (((2 ^ 3) * 8)) imm);
+      BitVec.and rs1_val immext := by rfl
+
+
+-- 4 tried to prove addition
+/-theorem MUL_bitvec : execute_MUL_pure64 { high := false, signed_rs1 := false, signed_rs2 := false } (reg1 : BitVec 64) (reg2 : BitVec 64) = BitVec.mul reg2 reg1 := by
+  unfold execute_MUL_pure64
+  simp only [Bool.false_eq_true, ↓reduceIte, BitVec.mul_eq]
+  simp [Functions.xlen]
+  have h1 : (2 : Int) * (2 ^(3 : Int) * 8) = 128 := by rfl --such that types match
+  rw [h1]
+  simp [Sail.BitVec.extractLsb]
+  simp [to_bits]
+  simp [ get_slice_int]
+  simp [BitVec.extractLsb]
+  simp [extractLsb'_extractLsb'2]
+  unfold HPow.hPow
+  unfold instHPowInt_leanRV64DLEAN
+  simp
+  have h2: min 64 128 = 64 := by rfl
+  rw [h2]
+  unfold HMul.hMul
+  unfold HAdd.hAdd
+  unfold Int.instMax
+  sorry-/
